\documentclass[12pt,letterpaper]{article}
\usepackage{amsmath}
\usepackage{amsfonts}
\usepackage{amsthm}
\usepackage{mathtools}
\usepackage{cancel}
\usepackage[bottom=1in,left=0.5in,right=1in,top=1in]{geometry}
\usepackage{titling}

% From https://code.google.com/p/linear-algebra/source/browse/linalgjh.sty#80
% Using brackets instead of parens.

%-------------bmat
% For matrices with arguments.
% Usage: \begin{bmat}{c|c|c} 1 &2 &3 \end{bmat}
\newenvironment{bmat}[1]{
  \left[\begin{array}{@{}#1@{}}
}{\end{array}\right]
}

\newcommand\numberthis{\addtocounter{equation}{1}\tag{\theequation}}
\newcommand{\GLNR}[0]{GL_n(\mathbb{R})}
\newcommand{\KER}[1]{\text{ker }#1}
\newcommand{\IM}[1]{\text{im }#1}
\newcommand{\ghg}[1]{g#1g^{-1}}

\setlength{\droptitle}{-10ex}

\preauthor{\begin{flushright}\large \lineskip 0.5em}
\postauthor{\par\end{flushright}}
\predate{\begin{flushright}\large}
\postdate{\par\end{flushright}}

\title{MAT 150A Homework 7\vspace{-2ex}}
\author{Hardy Jones\\
        999397426\\
        Professor Schilling\vspace{-2ex}}
\date{Fall 2014}

\begin{document}
  \maketitle

  \begin{enumerate}
    \item
      \begin{proof}
        Assume $O_n \trianglelefteq M_n$ is a normal subgroup.

        Choose $g = t_a \rho_\theta r, g^{-1} = t_{-a} \rho_{-\theta} r \in M_n, h = \rho_\psi r \in O_n$.

        Then we should have $\ghg{h} \in O_n$.

        \begin{align*}
          \ghg{h} &= t_a \rho_\theta (r \rho_\psi) t_{-a} \rho_{-\theta} r \\
          &= t_a \rho_\theta \rho_{-\psi} (r t_{-a}) \rho_{-\theta} r \\
          &= t_a \rho_\theta \rho_{-\psi} t_{-a'} (r \rho_{-\theta}) r \\
          &= t_a \rho_\theta \rho_{-\psi} t_{-a'} \rho_\theta r^2 \\
          &= t_a \rho_\theta (\rho_{-\psi} t_{-a'}) \rho_\theta \\
          &= t_a (\rho_\theta t_{-a''}) \rho_{-\psi} \rho_\theta \\
          &= (t_a t_{-a'''}) (\rho_\theta \rho_{-\psi} \rho_\theta) \\
          &= t_{a - a'''} \rho_{\theta - \psi + \theta} \\
        \end{align*}

        However, there's no guarantee that $a - a''' = 0$,
        so this may be a translation, which is not an orthogonal matrix.

        So, $\ghg{h} \notin O_n$, and our assumption is wrong.

        Thus,  $O_n$ is not a normal subgroup of $M_n$.
      \end{proof}

    \item
      \begin{proof}
        Let $m = t_a \rho_\theta r$
        \begin{align*}
          m^2 &= (t_a \rho_\theta r)(t_a \rho_\theta r) \\
          &= t_a \rho_\theta (rt_a) \rho_\theta r \\
          &= t_a \rho_\theta (t_{a'}r) \rho_\theta r \\
          &= t_a \rho_\theta t_{a'}(r \rho_\theta) r \\
          &= t_a \rho_\theta t_{a'}( \rho_{-\theta} r) r \\
          &= t_a \rho_\theta t_{a'} \rho_{-\theta} r^2 \\
          &= t_a (\rho_\theta t_{a'}) \rho_{-\theta} \\
          &= t_a (t_{a''} \rho_\theta) \rho_{-\theta} \\
          &= t_a t_{a''} (\rho_\theta \rho_{-\theta}) \\
          &= t_a t_{a''} (\rho_{\theta - \theta}) \\
          &= t_a t_{a''} \\
          &= t_{a + a''} \\
        \end{align*}

        So $m^2$ is just a translation by $a + a''$,
        where $a'' = \rho(r(a))$
      \end{proof}
    \item
      To show this, we need to show first that $SM \le M$ is a subgroup, and then $SM \trianglelefteq M$ is normal.

      Where $SM = \{t_a \rho_\theta r | \left| \rho_\theta r \right| = 1\}, M = \{t_a \rho_\theta r | \left| \rho_\theta r \right| = \pm 1\}$.

      And
      \[
        \rho_\theta(x) =
        \begin{bmatrix}
          \cos{\theta} & -\sin{\theta} \\
          \sin{\theta} & \cos{\theta}
        \end{bmatrix}
        \begin{bmatrix}
          x_1 \\
          x_2
        \end{bmatrix}
      \]

      \begin{proof}

        We first note that $\forall a = t_a \rho_\theta r \in SM, |r| = 1$ implies that there is no reflection.
        So for the sake of brevity, it is not included unless necessary.

        This also implies that $|\rho_\theta| = 1$ for all elements of $SM$.
        \begin{itemize}
          \item \textbf{Closure}

            Choose $a = t_a \rho_\theta, b = t_b \rho_\psi \in SM$

            \[
              ab = t_a \rho_\theta t_b \rho_\psi = t_a t_b \rho_\theta \rho_\psi = t_{a + b} \rho_{\theta + \psi}
            \]

            So we want to find
            \[
              \begin{vmatrix}
                \cos{\theta + \psi} & -\sin{\theta + \psi}
                \sin{\theta + \psi} & \cos{\theta + \psi}
              \end{vmatrix}
              = \cos^2(\theta + \psi) + \sin^2(\theta + \psi)
              = 1
            \]

            Thus $SM$ has closure.

          \item \textbf{Identity}

            Choose $a = 0 \in \mathbb{R}^n, \theta = 0 \in \mathbb{R}$,
            so $e = t_0 \rho_0$ and

            \[
              \begin{vmatrix}
                \cos{0} & -\sin{0} \\
                \sin{0} & \cos{0}
              \end{vmatrix}
              =
              \begin{vmatrix}
                1 & 0 \\
                0 & 1
              \end{vmatrix}
              = 1
            \]

            Now, choose $b = t_b \rho_\psi \in SM$.

            \[
              be = t_b \rho_\psi t_0 \rho_0 = t_b t_0 \rho_\psi \rho_0 = t_{b + 0} \rho_{\psi + 0} = t_b \rho_\psi = t_{0 + b} \rho_{0 + \psi} = t_0 t_b \rho_0 \rho_\psi = t_0 \rho_0 t_b \rho_\psi = eb
            \]

            Thus, $SM$ has the identity.

          \item \textbf{Inverse}

            Choose $a = t_a \rho_\theta \in SM$.
            Since $-a \in \mathbb{R}^n, -\theta \in \mathbb{R}$ exist,
            $a^{-1} = t_{-a} \rho_{-\theta} \in SM$.

            \[
              \begin{bmatrix}
                \cos{-\theta} & -\sin{-\theta} \\
                \sin{-\theta} & \cos{-\theta}
              \end{bmatrix}
              =
              \begin{bmatrix}
                \cos{\theta} & \sin{\theta} \\
                -\sin{\theta} & \cos{\theta}
              \end{bmatrix}
            \]

            \begin{align*}
              aa^{-1} &= t_a \rho_\theta t_{-a} \rho_{-\theta} \\
              &= t_a t_{-a} \rho_\theta \rho_{-\theta}  \\
              &= t_{a - a} \rho_{\theta - \theta}  \\
              &= t_0 \rho_0  \\
              &= e  \\
              &= t_{(- a) + a} \rho_{(-\theta) + \theta}  \\
              &= t_{-a} t_a \rho_{-\theta} \rho_\theta  \\
              &= t_{-a} \rho_{-\theta} t_a \rho_\theta  \\
              &= a^{-1}a \\
            \end{align*}
        \end{itemize}

        So, $SM \le M$ is a subgroup.

        Now we need to show that $SM \trianglelefteq M$ is normal.

        Choose an arbitrary $g = t_g \rho_\theta \in SM, h = t_h \rho_\psi r \in M$.

        \begin{align*}
          \ghg{h} &= t_g \rho_\theta (t_h \rho_\psi r) t_{-g} \rho_{-\theta} \\
          &= t_g (\rho_\theta t_h) \rho_\psi r t_{-g} \rho_{-\theta} \\
          &= t_g (t_h' \rho_\theta) \rho_\psi r t_{-g} \rho_{-\theta} \\
          &= (t_g t_h') (\rho_\theta \rho_\psi) r t_{-g} \rho_{-\theta} \\
          &= t_{g + h'} \rho_{\theta + \psi} r t_{-g} \rho_{-\theta} \\
          &= t_{g + h'} \rho_{\theta + \psi} (t_{-g'} r) \rho_{-\theta} \\
          &= t_{g + h'} \rho_{\theta + \psi} t_{-g'} (\rho_\theta r) \\
          &= t_{g + h'} \rho_{\theta + \psi} t_{-g'} (\rho_\theta r) \\
        \end{align*}
      \end{proof}
    \item
      We choose a homomorphism
      \[
        \varphi : SM \rightarrow GL_2(\mathbb{C})
      \]
      \[
        \varphi(t_a\rho_\theta) \mapsto
        \begin{bmatrix}
          e^{i \theta} & a_1 + i a_2 \\
          0 & 1
        \end{bmatrix}
      \]

      We need to show that $\varphi$ preserves the group operation.

      Choose $a = t_a \rho_\theta, b = t_b \rho_\psi \in SM$.

      \begin{align*}
        \varphi(a)\varphi(b) &=
        \begin{bmatrix}
          e^{i \theta} & a_1 + i a_2 \\
          0 & 1
        \end{bmatrix}
        \begin{bmatrix}
          e^{i \psi} & b_1 + i b_2 \\
          0 & 1
        \end{bmatrix} \\
        &=
        \begin{bmatrix}
          e^{i \theta} & a_1 + i a_2 \\
          0 & 1
        \end{bmatrix}
      \end{align*}
    \item
    \item
      \begin{enumerate}
        \item
        \item
        \item
      \end{enumerate}
  \end{enumerate}
\end{document}
