\documentclass[12pt,letterpaper]{article}
\usepackage{amsmath}
\usepackage{amsfonts}
\usepackage{amsthm}
\usepackage{cancel}
\usepackage[margin=1in]{geometry}
\usepackage{titling}

\setlength{\droptitle}{-10ex}

\preauthor{\begin{flushright}\large \lineskip 0.5em}
\postauthor{\par\end{flushright}}
\predate{\begin{flushright}\large}
\postdate{\par\end{flushright}}

\title{MAT 167 Homework 2\vspace{-2ex}}
\author{Hardy Jones\\
        999397426\\
        Professor Cheer\vspace{-2ex}}
\date{Winter 2014}

\begin{document}
  \maketitle

  \section*{1.7}
    \subsection*{4}
      Write down the 3 by 3 finite-difference matrix equation ($h = \frac{1}{4}$) for
      \[-\frac{d^2u}{dx^2} + u = x, \qquad u(0) = u(1) = 0\].

      Following from the text

      \[\frac{d^2u}{dx^2} \approx \frac{\Delta^2u}{\Delta x^2} = \frac{u(x+h) - 2u(x) + u(x-h)}{h^2}\]

      So we have

      \[-\frac{u(x+h) - 2u(x) + u(x-h)}{h^2} + u = x\]

      Letting $x = jh$, and realizing that $u$ must be a function of $x$

      \begin{align*}
        -\frac{u(jh+h) - 2u(jh) + u(jh-h)}{h^2} + u(jh) &= jh \\
        -\frac{u((j+1)h) - 2u(jh) + u((j-1)h)}{h^2} + u(jh) &= jh \\
        -u((j+1)h) + 2u(jh) - u((j-1)h) + u(jh)h^2 &= jh^3
      \end{align*}

      We take another cue from the text and use the notation $u(jh) = u_j$
      \begin{align*}
        -u_{j+1} + 2u_j - u_{j-1} + u_jh^2 &= jh^3 \\
        -u_{j+1} + u_jh^2 + 2u_j - u_{j-1} &= jh^3 \\
        -u_{j+1} + (h^2 + 2)u_j - u_{j-1} &= jh^3
      \end{align*}

      Since we have $h = \frac{1}{4}$

      \begin{align*}
        -u_{j+1} + ((\tfrac{1}{4})^2 + 2)u_j - u_{j-1} &= j(\tfrac{1}{4})^3 \\
        -u_{j+1} + (\tfrac{1}{16} + 2)u_j - u_{j-1} &= \tfrac{j}{64}
        -u_{j+1} + \tfrac{33}{16}u_j - u_{j-1} &= \tfrac{j}{64}
      \end{align*}

      Now we check each of $j = 1,2,3$, remembering $u(0) = u_0 = u(1) = u_4 = 0$

      $j = 1$
      \begin{align*}
        -u_{1+1} + \tfrac{33}{16}u_1 - u_{1-1} &= \tfrac{1}{64} \\
        -u_2 + \tfrac{33}{16}u_1 - u_0 &= \tfrac{1}{64} \\
        -u_2 + \tfrac{33}{16}u_1 &= \tfrac{1}{64}
      \end{align*}

      $j = 2$
      \begin{align*}
        -u_{2+1} + \tfrac{33}{16}u_2 - u_{2-1} &= \tfrac{2}{64} \\
        -u_{3} + \tfrac{33}{16}u_2 - u_{1} &= \tfrac{2}{64}
      \end{align*}

      $j = 3$
      \begin{align*}
        -u_{3+1} + \tfrac{33}{16}u_3 - u_{3-1} &= \tfrac{3}{64} \\
        -u_{4} + \tfrac{33}{16}u_3 - u_{2} &= \tfrac{3}{64} \\
        \tfrac{33}{16}u_3 - u_{2} &= \tfrac{3}{64}
      \end{align*}

      So we have
      \begin{align*}
        -u_2 + \tfrac{33}{16}u_1 &= \tfrac{1}{64} \\
        -u_{3} + \tfrac{33}{16}u_2 - u_{1} &= \tfrac{2}{64} \\
        \tfrac{33}{16}u_3 - u_{2} &= \tfrac{3}{64}
      \end{align*}

      Rearranging
      \begin{align*}
        \tfrac{33}{16}u_1 - u_2 &= \tfrac{1}{64} \\
        -u_{1} + \tfrac{33}{16}u_2 - u_{3}&= \tfrac{2}{64} \\
        -u_{2} + \tfrac{33}{16}u_3 &= \tfrac{3}{64}
      \end{align*}

      \[
        \left[
        \begin{array}{ccc}
        \tfrac{33}{16} & -1             & 0              \\
        -1             & \tfrac{33}{16} & -1             \\
        0              & -1             & \tfrac{33}{16}
        \end{array}
        \right]
        \left[
        \begin{array}{c}
        u_1 \\
        u_2 \\
        u_3
        \end{array}
        \right]
        =
        \frac{1}{64}
        \left[
        \begin{array}{c}
        1 \\
        2 \\
        3
        \end{array}
        \right]
      \]
    \subsection*{8}
    \subsection*{10}

  \section*{2.1}
    \subsection*{4}
    \subsection*{5}
    \subsection*{10}
    \subsection*{24}
    \subsection*{28}

  \section*{2.2}
    \subsection*{6}
    \subsection*{13}
    \subsection*{25}
    \subsection*{30}
    \subsection*{39}
    \subsection*{53}

  \section*{2.3}
    \subsection*{8}
    \subsection*{16}
    \subsection*{20}
    \subsection*{26}
    \subsection*{30}
    \subsection*{42}
\end{document}
